\documentclass{article}
\usepackage{amsthm, amssymb, amsmath}

\newtheorem{theorem}{Theorem}

\begin{document}

\begin{theorem}[Mean Value Theorem]
Let \( f : [a, b] \to \mathbb{R} \) be a function that is continuous on the closed interval \([a, b]\) and differentiable on the open interval \((a, b)\). Then there exists some \( c \in (a, b) \) such that:

\[
f'(c) = \frac{f(b) - f(a)}{b - a}
\]
\end{theorem}

\begin{proof}
Define the auxiliary function:

\[
g(x) = f(x) - \left( \frac{f(b) - f(a)}{b - a} \right)(x - a)
\]

Notice that \( g \) is continuous on \([a, b]\) and differentiable on \((a, b)\), because \( f \) is and the other terms are polynomials. Moreover,

\[
g(a) = f(a)
\]
\[
g(b) = f(b) - \left( \frac{f(b) - f(a)}{b - a} \right)(b - a) = f(b) - (f(b) - f(a)) = f(a)
\]

Thus, \( g(a) = g(b) \). By Rolle's Theorem, there exists some \( c \in (a, b) \) such that \( g'(c) = 0 \).

Calculating \( g'(x) \):

\[
g'(x) = f'(x) - \left( \frac{f(b) - f(a)}{b - a} \right)
\]

Setting \( g'(c) = 0 \) gives:

\[
f'(c) = \frac{f(b) - f(a)}{b - a}
\]

as desired. \qedhere
\end{proof}

\end{document}